src/coq/fool/Dot_Syntax.v
@@ -3,28 +3,25 @@
 Require Export Dot_Labels.
 Require Import Metatheory.
 
-Definition loc := var.
-
 Inductive tp : Set :=                         (* Type *)                 (* S, T, U, V *)
-  | tp_sel : pt -> label -> tp                  (* type selection *)       (* p.L *)
+  | tp_sel : tm -> label -> tp                  (* type selection *)       (* p.L *)
   | tp_rfn : tp -> list (label * decl) -> tp    (* refinement *)           (* T { z => Ds } *)
+(*| tp_fun : tp -> tp -> tp                     (* function type *)        (* T -> T *)*)
   | tp_and : tp -> tp -> tp                     (* intersection type *)    (* T /\ T *)
   | tp_or  : tp -> tp -> tp                     (* union type *)           (* T \/ T *)
   | tp_top : tp                                 (* top type *)             (* ⊤ *)
   | tp_bot : tp                                 (* bottom type *)          (* ⊥ *)
 
-with pt : Set :=                              (* Path *)                 (* p *)
-                                                (* Variables *)            (* x, y, z *)
-  | bvar : nat -> pt                            (* bound variable *)
-  | fvar : var -> pt                            (* free variable *)
-  | ref  : loc -> pt                            (* object reference *)     (* o *)
-  | sel  : pt -> label -> pt                    (* selection *)            (* p.l *)
-
 with tm : Set :=                              (* Term *)                 (* t *)
-  | path : pt -> tm
+                                                (* Variables *)            (* x, y, z *)
+  | bvar : nat -> tm                            (* bound variable *)
+  | fvar : var -> tm                            (* free variable *)
+(*| ref  : loc -> tm                            (* object reference *)*)
+(*| lam  : tp -> tm -> tm                       (* function *)             (* λx:T.t *)*)
+(*| app  : tm -> tm -> tm                       (* application *)          (* t t *)*)
   | new  : tp -> list (label * tm) -> tm -> tm  (* new instance *)         (* val x = new c; t *)
-  | msg : pt -> label -> pt -> tm -> tm         (* method invocation *)    (* val x = p.m(p); t *)
-  | exe : loc -> label -> tm -> tm -> tm        (* pending met. exec *)    (* val x = o.m... t; t *)
+  | sel  : tm -> label -> tm                    (* selection *)            (* t.l *)
+  | msel : tm -> label -> tm -> tm              (* method invocation *)    (* t m t *)
 
 with decl : Set :=                            (* Declaration *)          (* D *)
   | decl_tp : tp -> tp -> decl                  (* type declaration *)     (* L : S .. U *)
@@ -32,9 +29,15 @@ with decl : Set :=                            (* Declaration *)          (* D *)
   | decl_mt : tp -> tp -> decl                  (* method declaration *)   (* m : S -> U *)
 .
 
+Inductive path : tm -> Prop :=
+  | path_bvar : forall a, path (bvar a)
+  | path_fvar : forall a, path (fvar a)
+  | path_sel  : forall p l, path p -> value_label l -> path (sel p l)
+.
+
 Inductive concrete : tp -> Prop :=
   | concrete_sel : forall p lc,
-      concrete_label lc -> concrete (tp_sel p lc)
+      path p -> concrete_label lc -> concrete (tp_sel p lc)
   | concrete_rfn : forall tc ds,
       concrete tc -> concrete (tp_rfn tc ds)
   | concrete_and : forall t1 t2,
@@ -46,13 +49,12 @@ Inductive concrete : tp -> Prop :=
 Definition args := list (label * tm).
 Definition decls_lst := list (label * decl).
 
-Definition store : Set := list (loc * (tp * args)).
-Definition gamma : Set := list (var * tp).
-Definition env : Set := (gamma * store)%type.
-Definition ctx_bind (E: env) (x: var) (T: tp) : env := match E with (g,p) => (((x ~ T) ++ g),p) end.
+Definition store : Set := list (var * (tp * args)).
+Definition env : Set := list (var * tp).
+Definition ctx_bind (E: env) (x: var) (T: tp) : env := ((x ~ T) ++ E).
 
-Coercion bvar : nat >-> pt.
-Coercion fvar : var >-> pt.
+Coercion bvar : nat >-> tm.
+Coercion fvar : var >-> tm.
 
 (** * Automation *)
-Hint Constructors tp decl tm concrete.
+Hint Constructors tp decl tm path concrete.
