src/coq/fool/Dot_Labels.v
@@ -1,0 +1,106 @@
+(** The DOT calculus -- Labels. *)
+
+Require Import Metatheory.
+
+Inductive label : Set :=
+  | lv : atom -> label          (* Value label *)          (* l *)
+  | lm : atom -> label          (* Method label *)         (* m *)
+                                (* Type label *)           (* L *)
+  | lc : atom -> label            (* class label *)          (* Lc *)
+  | la : atom -> label            (* abstract type label *)  (* La *)
+.
+
+Inductive value_label : label -> Prop :=
+  | value_labe_lv : forall a, value_label (lv a)
+.
+
+Inductive method_label : label -> Prop :=
+  | method_label_lm : forall a, method_label (lm a)
+.
+
+Inductive type_label : label -> Prop :=
+  | type_label_lc : forall a, type_label (lc a)
+  | type_label_la : forall a, type_label (la a)
+.
+
+Inductive concrete_label : label -> Prop :=
+  | concrete_label_lc : forall a, concrete_label (lc a)
+.
+
+Require Import Coq.Classes.EquivDec.
+Require Import Coq.Program.Program.
+
+Program Instance eq_label_dec : @EqDec label eq eq_equivalence :=
+  { equiv_dec x y :=
+    match x, y with
+      | lv n, lv n' => if n == n' then in_left else in_right
+      | lm n, lm n' => if n == n' then in_left else in_right
+      | la n, la n' => if n == n' then in_left else in_right
+      | lc n, lc n' => if n == n' then in_left else in_right
+      | lv n, lm n' | lm n, lv n' | lv n, la n' | la n, lv n' | lv n, lc n' | lc n, lv n' | lm n, la n' | la n, lm n' | lm n, lc n' | lc n, lm n' | la n, lc n' | lc n, la n'  => in_right (* why does wildcard pattern not work?*)
+    end }.
+  Obligation Tactic := unfold complement, equiv ; program_simpl.
+  Solve Obligations using unfold equiv, complement in * ; program_simpl ; intuition (discriminate || eauto).
+
+Instance EqDec_label : @EqDec label eq eq_equivalence.
+Proof. exact eq_label_dec. Defined.
+
+Module LabelDT <: UsualDecidableType with Definition t := label.
+  Definition t := label.
+
+  Definition eq := @eq t.
+  Definition eq_refl := @refl_equal t.
+  Definition eq_sym := @sym_eq t.
+  Definition eq_trans := @trans_eq t.
+
+  Definition eq_dec := eq_label_dec.
+End LabelDT.
+
+Module Import LabelSetImpl : FSetExtra.WSfun LabelDT := FSetExtra.Make LabelDT.
+Notation labels := LabelSetImpl.t.
+Module Export LabelSetDecide := CoqFSetDecide.WDecide_fun LabelDT LabelSetImpl.
+Module Export LabelSetFacts := FSetFacts.WFacts_fun LabelDT LabelSetImpl.
+Module LabelSetProperties := FSetProperties.WProperties_fun LabelDT LabelSetImpl.
+
+Notation "s [=l=] t" := (LabelSetImpl.Equal s t) (at level 70, no associativity).
+Notation "s  [<l=]  t" := (LabelSetImpl.Subset s t) (at level 70, no associativity).
+
+Module Export LabelMapImpl := AssocList.Make LabelDT LabelSetImpl.
+
+Ltac simpl_labelmap := simpl_alist.
+
+Tactic Notation "simpl_labelmap" "in" hyp(H) :=
+  simpl_alist in H.
+
+Tactic Notation "simpl_labelmap" "in" "*" :=
+  simpl_alist in *.
+
+Tactic Notation "rewrite_labelmap" constr(E) :=
+  rewrite_alist E.
+
+Tactic Notation "rewrite_labelmap" constr(E) "in" hyp(H) :=
+  rewrite_alist E in H.
+
+Tactic Notation "labelmap" "induction" ident(E) :=
+  alist induction E.
+
+Tactic Notation "labelmap" "induction" ident(E) "as" simple_intropattern(P) :=
+  alist induction E as P.
+
+Notation uniq_one := uniq_one_1.
+Notation uniq_cons := uniq_cons_3.
+Notation uniq_app := uniq_app_4.
+Notation uniq_map := uniq_map_2.
+
+Notation binds_one := binds_one_3.
+Notation binds_cons := binds_cons_3.
+Notation binds_app_l := binds_app_2.
+Notation binds_app_r := binds_app_3.
+Notation binds_map := binds_map_2.
+
+Hint Resolve
+  LabelSetImpl.add_1 LabelSetImpl.add_2 LabelSetImpl.remove_1
+  LabelSetImpl.remove_2 LabelSetImpl.singleton_2 LabelSetImpl.union_2
+  LabelSetImpl.union_3 LabelSetImpl.inter_3 LabelSetImpl.diff_3.
+
+Module lbl := LabelMapImpl.
