src/coq/fool/Dot_Lemmas.v
@@ -10,11 +10,54 @@ Require Import Coq.Classes.Equivalence.
 Require Import Coq.Classes.EquivDec.
 Require Import Coq.Logic.Decidable.
 
+(* ********************************************************************** *)
+(** ** Evaluation *)
+
+Lemma ev_wf_store : forall s s' t t',
+  s |~ t ~>~ t' ~| s' -> wf_store s /\ wf_store s'.
+Proof.
+  introv H. split.
+    induction H; try assumption.
+      Case "ev_new".
+        inversion IHev; subst. assumption.
+    induction H; try assumption.
+Qed.
+
 Lemma value_xor_method_label : forall l,
   value_label l -> method_label l -> False.
 Proof.
   introv Hvalue Hmethod. inversion Hvalue. inversion Hmethod.
   rewrite <- H0 in H. inversion H.
+Qed.
+
+Lemma wf_store_lbl_binds_value : forall s l v a Tc ags,
+  wf_store s -> binds a (Tc, ags) s -> lbl.binds l v ags -> value_label l -> value v.
+Proof.
+  introv Hwf Hb Hlb Hvalue. induction Hwf.
+  Case "nil". inversion Hb.
+  Case "rest".
+   rewrite_env ((x, (Tc0, args))::E) in Hb.
+   apply binds_cons_1 in Hb. inversions Hb.
+   SCase "x = a ".
+     inversions H3. inversions H5. 
+     remember (H l v Hlb) as H'.
+     inversions H'.
+       inversions H3. assumption.
+       assert False as Contra. apply value_xor_method_label with (l:=l); assumption. inversion Contra.
+   SCase "x <> a".
+     apply IHHwf.
+     assumption.
+Qed.
+
+Lemma ev_to_value : forall s s' t v,
+  s |~ t ~>~ v ~| s' -> value v.
+Proof.
+  introv H. induction H; try assumption.
+    Case "ev_sel".
+      inversion H2; subst.
+        apply wf_store_lbl_binds_value with (s:=sf) (l:=lv a0) (a:=a) (Tc:=Tc) (ags:=ags);
+        try apply (proj2 (ev_wf_store H));
+        assumption.
 Qed.
 
 (* ********************************************************************** *)
@@ -61,16 +104,15 @@ Lemma expansion_decls_ok : forall E T DS,
 Proof.
   introv H. induction H. induction H; try solve [
     apply decls_ok_fin_nil |
-    inversion H; assumption |
     inversion H0; assumption |
     inversion H1; assumption].
 Qed.
 Hint Resolve expansion_decls_ok.
 
-Lemma expands_bot_inf_nil : forall E, E |= tp_bot ~< decls_inf nil.
+Lemma expands_bot_inf_nil : forall E, wf_env E -> E |= tp_bot ~< decls_inf nil.
 Proof.
   Hint Constructors bot_decl valid_label.
-  intros E.
+  introv Henv.
   apply expands_any. apply expands_iter_bot; auto.
   Case "bot_decls (decls_inf nil)". unfold bot_decls. splits.
     SCase "decls_ok (decls_inf nil)". unfold decls_ok. splits.
@@ -97,16 +139,17 @@ Qed.
 (* ********************************************************************** *)
 (** ** Well-formedness *)
 
-Lemma wfe_bot : forall E,  wfe_tp E tp_bot.
+Lemma wfe_bot : forall E, wf_env E -> wfe_tp E tp_bot.
 Proof.
   Hint Constructors bot_decl.
-  intros E. apply wfe_any with (DT:=decls_inf nil); auto using wf_bot.
+  introv Henv.
+  apply wfe_any with (DT:=decls_inf nil); auto using wf_bot.
 Qed.
 Hint Resolve wfe_bot.
 
-Lemma wfe_top : forall E, wfe_tp E tp_top.
+Lemma wfe_top : forall E, wf_env E -> wfe_tp E tp_top.
 Proof.
-  intros E.
+  introv Henv.
   apply wfe_any with (DT:=decls_fin nil); auto using wf_top, expands_any, expands_iter_top.
 Qed.
 Hint Resolve wfe_top.
@@ -121,14 +164,24 @@ Ltac add_expands_hyp E T DT HxT :=
 
 Lemma sub_tp_regular : forall E S T,
   E |= S ~<: T ->
-  wfe_tp E S /\ wfe_tp E T.
+  wf_env E /\ wfe_tp E S /\ wfe_tp E T.
 Proof.
 
+Hint Extern 1 (wf_env ?E) =>
+  match goal with
+  | IH: wf_env ?E /\ _ /\ _ |- _ => apply (proj1 IH)
+  end.
 Hint Extern 1 (wfe_tp ?E ?T) =>
   match goal with
-  | IH: wfe_tp ?E ?T /\ _ |- _ => apply (proj1 IH)
-  | IH: _ /\ wfe_tp ?E ?T |- _ => apply (proj2 IH)
+  | IH: _ /\ wfe_tp ?E ?T /\ _ |- _ => apply (proj1 (proj2 IH))
+  | IH: _ /\ _ /\ wfe_tp ?E ?T |- _ => apply (proj2 (proj2 IH))
   end.
+
+(* Hint Extern 2 (wfe_tp ?E (tp_sel ?p ?L)) =>
+  match goal with
+  | H: ?E |= ?p ~mem~ ?L ~: decl_tp ?S ?U |- _ => let DU := fresh "DU" with HxU := fresh "HxU" in
+    add_expands_hyp E U DU HxU; inversion HxU; subst; apply wfe_any with (DT:=DU); eauto 3
+  end. *)
 
 Ltac combine_decls E T1 T2 DSM cmb_decls decls_cmb_exists :=
   let DT1 := fresh "DT1" with HxT1 := fresh "HxT1" with DT2 := fresh "DT2" with HxT2 := fresh "HxT2"
@@ -150,12 +203,12 @@ Hint Constructors wf_tp expands expands_iter.
 Hint Extern 1 (wf_tp ?E ?T) =>
   match goal with
   | IH: wfe_tp ?E ?T |- _ => inversion IH; subst; assumption
-  | IH: wfe_tp ?E ?T /\ _ |- _ =>
+  | IH: _ /\ wfe_tp ?E ?T /\ _ |- _ =>
     let Hwfe := fresh "Hwfe" in (assert (wfe_tp E T) as Hwfe);
-      try apply (proj1 IH); inversion Hwfe; assumption
-  | IH: _ /\ wfe_tp ?E ?T |- _ =>
+      try apply (proj1 (proj2 IH)); inversion Hwfe; assumption
+  | IH: _ /\ _ /\ wfe_tp ?E ?T |- _ =>
     let Hwfe := fresh "Hwfe" in (assert (wfe_tp E T) as Hwfe);
-      try apply (proj2 IH); inversion Hwfe; assumption
+      try apply (proj2 (proj2 IH)); inversion Hwfe; assumption
   end.
 
   introv H. induction H; splits; eauto 3.
@@ -163,10 +216,20 @@ Qed.
 
 (* *********************************************************************** *)
 (** * #<a name="auto"></a># Automation *)
+    
+Hint Extern 1 (wf_env ?E) =>
+  match goal with
+  | H: sub_tp _ _ _ |- _ => apply (proj1 (sub_tp_regular H))
+  end.
 
 Hint Extern 1 (wfe_tp ?E ?T) =>
   match goal with
-  | H: sub_tp E T _ |- _ => apply (proj1 (sub_tp_regular H))
-  | H: sub_tp E _ T |- _ => apply (proj2 (sub_tp_regular H))
+  | H: sub_tp E T _ |- _ => apply (proj1 (proj2 (sub_tp_regular H)))
+  | H: sub_tp E _ T |- _ => apply (proj2 (proj2 (sub_tp_regular H)))
   end.
 
+(*
+*** Local Variables:
+*** coq-load-path: ("metalib" "lib")
+*** End:
+*)
