src/coq/fool/Dot_Theorems.v
@@ -1,0 +1,124 @@
+(** The DOT calculus -- Theorems *)
+
+Set Implicit Arguments.
+Require Import List.
+Require Export Dot_Labels.
+Require Import Metatheory LibTactics_sf.
+Require Export Dot_Syntax Dot_Definitions Dot_Rules Dot_Lemmas.
+Require Import Coq.Program.Equality.
+Require Import Coq.Classes.Equivalence.
+Require Import Coq.Classes.EquivDec.
+Require Import Coq.Logic.Decidable.
+
+(* ********************************************************************** *)
+
+Scheme h_expands_iter_indm   := Induction for expands_iter Sort Prop
+  with h_expands_fix_indm    := Induction for expands_fix Sort Prop
+.
+
+Combined Scheme h_expands_mutind from h_expands_iter_indm, h_expands_fix_indm.
+Ltac mutind_h_expands P1_ P2_ :=
+  cut ((forall M E T DS (H: expands_iter M E T DS), (P1_ M E T DS H)) /\
+       (forall Ts Ds M E T DS (H: expands_fix Ts Ds M E T DS), (P2_ Ts Ds M E T DS H))); [tauto |
+    apply (h_expands_mutind P1_ P2_); try unfold P1_, P2_; [
+Case "expands_iter_rfn" | Case "expands_iter_tsel_cache" | Case "expands_iter_tsel_fix" | Case "expands_iter_and" | Case "expands_iter_or" | Case "expands_iter_top" | Case "expands_iter_bot" | Case "expands_fix_one" | Case "expands_fix_rec"];
+      introv; eauto ].
+
+Section TestHMutInd.
+  Let Pexi (M: list (tp * decls)) (E: env) (T: tp) (DS : decls) (H: expands_iter M E T DS) := True.
+  Let Pexf (Ts: tp) (Ds: decls) (M: list (tp * decls)) (E: env) (T: tp) (DS : decls) (H: expands_fix Ts Ds M E T DS) := True.
+Lemma EnsureMutindHExpandsTacticIsUpToDate : True.
+Proof. mutind_h_expands Pexi Pexf; intros; auto. Qed.
+End TestHMutInd.
+
+Section ExpansionOK.
+  Let P1_ (M': list (tp * decls)) (E': env) (T': tp) (DS' : decls) (H': expands_iter M' E' T' DS') :=
+    decls_ok DS'.
+  Let P2_ (Ts': tp) (Ds': decls) (M': list (tp * decls)) (E': env) (T': tp) (DS': decls) (H': expands_fix Ts' Ds' M' E' T' DS') :=
+    decls_ok DS'.
+
+  Lemma h_expands_decls_ok:
+    (forall (M': list (tp * decls)) (E': env) (T': tp) (DS' : decls) (H': expands_iter M' E' T' DS'), 
+     decls_ok DS')
+    /\
+    (forall (Ts': tp) (Ds': decls) (M': list (tp * decls)) (E': env) (T': tp) (DS': decls) (H': expands_fix Ts' Ds' M' E' T' DS'),
+     decls_ok DS').
+  Proof.
+    mutind_h_expands P1_ P2_.
+    Case "expands_iter_rfn".
+      intros Hexp Hok Hand. inversion Hand. assumption.
+    Case "expands_iter_and".
+      intros Hexp1 Hok1 Hexp2 Hok2 Hand. inversion Hand. assumption.
+    Case "expands_iter_or".
+      intros Hexp1 Hok1 Hexp2 Hok2 Hor. inversion Hor. assumption.
+  Qed.
+End ExpansionOK.
+
+Lemma tp_sel__expands_fix : forall p L E U,
+  exists DT,  expands_fix (tp_sel p L) (decls_fin nil) nil E U DT /\ decls_ok DT.
+Proof.
+  intros p L E U.
+  assert (exists DS, expands_iter ((tp_sel p L ~ (decls_fin nil)) ++ nil) E U DS /\ decls_ok DS) as Hfix1.
+    (* TODO *) skip.
+  assert (forall P, P \/ ~P) as HMid. skip.
+  inversion Hfix1 as [DS [HDSex HDSok]].
+  specialize (HMid (decls_fin nil = DS)). inversion HMid as [Heq | Hneq].
+  exists DS. rewrite Heq. split. apply expands_fix_one. rewrite Heq in HDSex. assumption. assumption.
+  assert (exists DSf, expands_fix (tp_sel p L) DS nil E U DSf /\ decls_ok DSf) as Hfix2.
+    (* TODO *) skip.
+  inversion Hfix2 as [DSf [HDSfex HDSfok]].
+  exists DSf. split. apply expands_fix_rec with (DSA:=DS). assumption. assumption. assumption. assumption.
+Qed.
+
+Theorem tp_wf__expands : forall E T,
+  wf_env E -> wf_tp E T -> exists DT, E |= T ~< DT.
+Proof.
+  intros E T Henv Hwf. induction Hwf.
+  Case "rfn".
+    specialize (IHHwf Henv). inversion IHHwf as [DT HDT].
+    assert (exists DSM, and_decls DT (decls_fin DS) DSM) as HDSM. apply decls_and_exists.
+      apply expansion_decls_ok in HDT. assumption. assumption.
+    inversion HDSM as [DSM HDSM'].
+    exists DSM.
+    apply expands_any. apply expands_iter_rfn with (DSP:=DT). inversion HDT; subst; assumption. assumption.
+  Case "sel".
+    assert (exists DT,  expands_fix (tp_sel p L) (decls_fin nil) nil E U DT /\ decls_ok DT) as Hfix.
+      apply tp_sel__expands_fix; auto.
+    inversion Hfix as [DT [HDTfix HDTok]].
+    exists DT.
+    apply expands_any. apply expands_iter_tsel_fix with (S:=S) (U:=U); auto.
+  Case "and".
+    specialize (IHHwf1 Henv). inversion IHHwf1 as [DT1 HDT1].
+    specialize (IHHwf2 Henv). inversion IHHwf2 as [DT2 HDT2].
+    assert (exists DSM, and_decls DT1 DT2 DSM) as HDSM. apply decls_and_exists.
+      apply expansion_decls_ok in HDT1. assumption.
+      apply expansion_decls_ok in HDT2. assumption.
+    inversion HDSM as [DSM HDSM'].
+    exists DSM.
+    apply expands_any. apply expands_iter_and with (DS1:=DT1) (DS2:=DT2).
+      inversion HDT1; subst; assumption.
+      inversion HDT2; subst; assumption.
+      assumption.
+  Case "or".
+    specialize (IHHwf1 Henv). inversion IHHwf1 as [DT1 HDT1].
+    specialize (IHHwf2 Henv). inversion IHHwf2 as [DT2 HDT2].
+    assert (exists DSM, or_decls DT1 DT2 DSM) as HDSM. apply decls_or_exists.
+      apply expansion_decls_ok in HDT1. assumption.
+      apply expansion_decls_ok in HDT2. assumption.
+    inversion HDSM as [DSM HDSM'].
+    exists DSM.
+    apply expands_any. apply expands_iter_or with (DS1:=DT1) (DS2:=DT2).
+      inversion HDT1; subst; assumption.
+      inversion HDT2; subst; assumption.
+      assumption.
+  Case "bot".
+    exists (decls_inf nil). apply expands_bot_inf_nil. assumption.
+  Case "top".
+    exists (decls_fin nil). apply expands_any. apply expands_iter_top. assumption.
+Qed.
+
+(*
+*** Local Variables:
+*** coq-load-path: ("metalib" "lib")
+*** End:
+*)
