src/coq/fool/.dir-locals.el
@@ -1,0 +1,1 @@
+((coq-mode . ((coq-prog-args . ("-emacs-U" "-I" "../metalib" "-I" "../lib")))))
