src/coq/fool/README.md
@@ -1,0 +1,4 @@
+DOT in Coq
+==========
+
+The FOOL 2012 model is implemented in this directory.
